wip new definition

Fsub_Soundness.v
@@ -25,6 +25,122 @@ Admitted.
 Local Lemma cheat_with : forall A B, A -> B.
 Admitted.
 
+
+(** Dealing with cv -- as a fixpoint is problematic. *)
+Inductive cvx : env -> typ -> captureset -> Prop :=
+  (** Looking up in the environment; we ask that T is wf in the environment
+      and that the environment is well formed so lookup is well defined. *)
+  | cvx_typ_var : forall (X : atom) T E CT,
+    binds X (bind_sub T) E ->
+    wf_env E ->
+    cvx E T CT ->
+    cvx E (typ_fvar X) CT
+  | cvx_typ_capt : forall E C P,
+    wf_env E ->
+    wf_pretyp_in E P ->
+    wf_cset_in E C ->
+    cvx E (typ_capt C P) C.
+
+
+(* HINT: we had problems formalizing a version with Ap and Am since then the
+   IH requires us to show wf_typ Ap Am, while we only have wf_typ_in E.
+ *)
+Lemma cv_unique_shrink : forall Y B E T C,
+  wf_env ([(Y, B)] ++ E) ->
+  wf_typ_in E T ->
+  cvx ([(Y, B)] ++ E) T C ->
+  cvx E T C.
+Proof.
+  intros*.
+  intros HwfE HwfT Hcv.
+
+  assert (type T). eapply type_from_wf_typ; eauto.
+
+  dependent induction Hcv.
+  * assert (X <> Y) by admit.
+    apply cvx_typ_var with (T := T).
+    unfold binds in H. unfold get in H. simpl in H.
+    destruct (X == Y) eqn:HXY; subst; trivial.
+    easy.
+
+    inversion HwfE; trivial.
+    eapply IHHcv with (Y0 := Y) (B0 := B).
+    inversion HwfT; subst.
+    admit.
+    trivial.
+    trivial.
+    admit.
+  * inversion HwfT; subst. constructor; trivial.
+    inversion H; trivial.
+Admitted.
+
+Lemma cv_unique : forall E T C1 C2,
+  wf_env E ->
+  wf_typ_in E T ->
+  cvx E T C1 ->
+  cvx E T C2 ->
+  C1 = C2.
+Proof with eauto*.
+  intros E; induction E; intros T; induction T; intros...
+  - inversion H1; inversion H2; subst...
+  - exfalso. inversion H0.
+  - exfalso.
+    inversion H0...
+    inversion H7...
+  - inversion H1...
+    inversion H2...
+  - inversion H0.
+  - destruct a as [Y B].
+    simpl_env in *.
+    destruct (Y == a0); subst...
+    + inversion H2; subst...
+      inversion H1; subst...
+      apply IHE with (T := T)...
+      {inversion H5; trivial. }
+      {binds_cases H4; subst; simpl_env in *; try notin_solve...
+        inversion H; trivial. }
+      {
+        binds_cases H4; subst; simpl_env in *; try notin_solve...
+        binds_cases H6; subst; simpl_env in *; try notin_solve...
+        inversion H6; subst...
+
+        eapply cv_unique_shrink.
+        apply H8.
+        inversion H. trivial.
+        trivial.
+      }
+      {
+        binds_cases H4; subst; simpl_env in *; try notin_solve...
+        binds_cases H6; subst; simpl_env in *; try notin_solve...
+        inversion H6; subst...
+
+        eapply cv_unique_shrink.
+        apply H8.
+        inversion H. trivial.
+        trivial.
+      }
+    + inversion H1; subst...
+      inversion H2; subst...
+      apply IHE with (T := a0)...
+      {inversion H5; trivial. }
+      {binds_cases H4; subst; simpl_env in *; try notin_solve...
+       }
+      {
+        eapply cv_unique_shrink.
+        apply H5.
+        binds_cases H4. eapply wf_typ_var.
+        apply H3.
+        apply H1.
+      }
+      {
+        eapply cv_unique_shrink.
+        apply H5.
+        binds_cases H4. eapply wf_typ_var.
+        apply H3.
+        apply H2.
+      }
+Qed.
+
 Lemma capt_from_cv : forall E T C,
     cv E T C -> capt C.
 Proof with eauto.
@@ -341,35 +457,6 @@ Proof with eauto*.
   inversion Hwf...
 Qed.
 
-(* HINT: we had problems formalizing a version with Ap and Am since then the
-   IH requires us to show wf_typ Ap Am, while we only have wf_typ_in E.
- *)
-Lemma cv_unique : forall E T C1 C2,
-  wf_env E ->
-  wf_typ_in E T ->
-  cv E T C1 ->
-  cv E T C2 ->
-  C1 = C2.
-Proof with eauto*.
-  intros E; induction E; intros T; induction T; intros...
-  - inversion H1; inversion H2; subst...
-  - exfalso. inversion H0.
-  - exfalso.
-    inversion H0...
-    inversion H7...
-  - inversion H1...
-    inversion H2...
-  - inversion H0.
-  - destruct a as [a' B].
-    simpl_env in *.
-    destruct (a' == a0); subst...
-    + inversion H2; subst...
-      inversion H1; subst...
-      apply IHE with (T := T)...
-    + inversion H1; subst...
-      inversion H2; subst...
-      apply IHE with (T := a0)...
-Qed.
 
 Lemma captures_transitivity : forall E xs ys x,
   (* E |- {x} <: {ys} *)
